Leanbin/Init/Data/Quot.lean
@@ -54,42 +54,40 @@ variable {r : α → α → Prop}
 
 variable {β : Quot r → Sort v}
 
--- ././Mathport/Syntax/Translate/Basic.lean:462:9: unsupported: advanced prec syntax max
-local notation:999 "⟦" a "⟧" => Quot.mk r a
+-- mathport name: «expr⟦ ⟧»
+local notation:arg "⟦" a "⟧" => Quot.mk r a
 
 @[reducible]
-protected def indepₓ (f : ∀ a, β (⟦a⟧)) (a : α) : Psigma β :=
+protected def indep (f : ∀ a, β ⟦a⟧) (a : α) : PSigma β :=
   ⟨⟦a⟧, f a⟩
 
-protected theorem indep_coherent (f : ∀ a, β (⟦a⟧))
-    (h : ∀ a b : α p : r a b, (Eq.ndrec (f a) (sound p) : β (⟦b⟧)) = f b) :
-    ∀ a b, r a b → Quot.indepₓ f a = Quot.indepₓ f b := fun a b e => Psigma.eq (sound e) (h a b e)
+protected theorem indep_coherent (f : ∀ a, β ⟦a⟧) (h : ∀ a b : α p : r a b, (Eq.ndrec (f a) (sound p) : β ⟦b⟧) = f b) :
+    ∀ a b, r a b → Quot.indep f a = Quot.indep f b := fun a b e => PSigma.eq (sound e) (h a b e)
 
-protected theorem lift_indep_pr1 (f : ∀ a, β (⟦a⟧))
-    (h : ∀ a b : α p : r a b, (Eq.ndrec (f a) (sound p) : β (⟦b⟧)) = f b) (q : Quot r) :
-    (lift (Quot.indepₓ f) (Quot.indep_coherent f h) q).1 = q :=
-  Quot.ind (fun a : α => Eq.refl (Quot.indepₓ f a).1) q
+protected theorem lift_indep_pr1 (f : ∀ a, β ⟦a⟧) (h : ∀ a b : α p : r a b, (Eq.ndrec (f a) (sound p) : β ⟦b⟧) = f b)
+    (q : Quot r) : (lift (Quot.indep f) (Quot.indep_coherent f h) q).1 = q :=
+  Quot.ind (fun a : α => Eq.refl (Quot.indep f a).1) q
 
 @[reducible, elab_as_eliminator]
-protected def recₓ (f : ∀ a, β (⟦a⟧)) (h : ∀ a b : α p : r a b, (Eq.ndrec (f a) (sound p) : β (⟦b⟧)) = f b)
-    (q : Quot r) : β q :=
-  Eq.recOnₓ (Quot.lift_indep_pr1 f h q) (lift (Quot.indepₓ f) (Quot.indep_coherent f h) q).2
+protected def rec (f : ∀ a, β ⟦a⟧) (h : ∀ a b : α p : r a b, (Eq.ndrec (f a) (sound p) : β ⟦b⟧) = f b) (q : Quot r) :
+    β q :=
+  Eq.recOnₓ (Quot.lift_indep_pr1 f h q) (lift (Quot.indep f) (Quot.indep_coherent f h) q).2
 
 @[reducible, elab_as_eliminator]
-protected def recOnₓ (q : Quot r) (f : ∀ a, β (⟦a⟧))
-    (h : ∀ a b : α p : r a b, (Eq.ndrec (f a) (sound p) : β (⟦b⟧)) = f b) : β q :=
-  Quot.recₓ f h q
+protected def recOn (q : Quot r) (f : ∀ a, β ⟦a⟧) (h : ∀ a b : α p : r a b, (Eq.ndrec (f a) (sound p) : β ⟦b⟧) = f b) :
+    β q :=
+  Quot.rec f h q
 
 @[reducible, elab_as_eliminator]
-protected def recOnSubsingletonₓ [h : ∀ a, Subsingleton (β (⟦a⟧))] (q : Quot r) (f : ∀ a, β (⟦a⟧)) : β q :=
-  Quot.recₓ f (fun a b h => Subsingleton.elimₓ _ (f b)) q
+protected def recOnSubsingleton [h : ∀ a, Subsingleton (β ⟦a⟧)] (q : Quot r) (f : ∀ a, β ⟦a⟧) : β q :=
+  Quot.rec f (fun a b h => Subsingleton.elimₓ _ (f b)) q
 
 @[reducible, elab_as_eliminator]
-protected def hrecOnₓ (q : Quot r) (f : ∀ a, β (⟦a⟧)) (c : ∀ a b : α p : r a b, HEq (f a) (f b)) : β q :=
-  Quot.recOnₓ q f fun a b p =>
+protected def hrecOn (q : Quot r) (f : ∀ a, β ⟦a⟧) (c : ∀ a b : α p : r a b, HEq (f a) (f b)) : β q :=
+  Quot.recOn q f fun a b p =>
     eq_of_heq
       (calc
-        HEq (Eq.ndrec (f a) (sound p) : β (⟦b⟧)) (f a) := eq_rec_heqₓ (sound p) (f a)
+        HEq (Eq.ndrec (f a) (sound p) : β ⟦b⟧) (f a) := eq_rec_heqₓ (sound p) (f a)
         HEq _ (f b) := c a b p
         )
 
@@ -105,8 +103,8 @@ namespace Quotientₓ
 protected def mk {α : Sort u} [s : Setoidₓ α] (a : α) : Quotientₓ s :=
   Quot.mk Setoidₓ.R a
 
--- ././Mathport/Syntax/Translate/Basic.lean:462:9: unsupported: advanced prec syntax max
-notation:999 "⟦" a "⟧" => Quotientₓ.mk a
+-- mathport name: «expr⟦ ⟧»
+notation:arg "⟦" a "⟧" => Quotientₓ.mk a
 
 theorem sound {α : Sort u} [s : Setoidₓ α] {a b : α} : a ≈ b → ⟦a⟧ = ⟦b⟧ :=
   Quot.sound
@@ -117,7 +115,7 @@ protected def lift {α : Sort u} {β : Sort v} [s : Setoidₓ α] (f : α → β
   Quot.lift f
 
 @[elab_as_eliminator]
-protected theorem ind {α : Sort u} [s : Setoidₓ α] {β : Quotientₓ s → Prop} : (∀ a, β (⟦a⟧)) → ∀ q, β q :=
+protected theorem ind {α : Sort u} [s : Setoidₓ α] {β : Quotientₓ s → Prop} : (∀ a, β ⟦a⟧) → ∀ q, β q :=
   Quot.ind
 
 @[reducible, elab_as_eliminator]
@@ -127,7 +125,7 @@ protected def liftOn {α : Sort u} {β : Sort v} [s : Setoidₓ α] (q : Quotien
 
 @[elab_as_eliminator]
 protected theorem induction_on {α : Sort u} [s : Setoidₓ α] {β : Quotientₓ s → Prop} (q : Quotientₓ s)
-    (h : ∀ a, β (⟦a⟧)) : β q :=
+    (h : ∀ a, β ⟦a⟧) : β q :=
   Quot.induction_on q h
 
 theorem exists_rep {α : Sort u} [s : Setoidₓ α] (q : Quotientₓ s) : ∃ a : α, ⟦a⟧ = q :=
@@ -141,22 +139,22 @@ variable [s : Setoidₓ α]
 
 variable {β : Quotientₓ s → Sort v}
 
-protected def rec (f : ∀ a, β (⟦a⟧)) (h : ∀ a b : α p : a ≈ b, (Eq.ndrec (f a) (Quotientₓ.sound p) : β (⟦b⟧)) = f b)
+protected def rec (f : ∀ a, β ⟦a⟧) (h : ∀ a b : α p : a ≈ b, (Eq.ndrec (f a) (Quotientₓ.sound p) : β ⟦b⟧) = f b)
     (q : Quotientₓ s) : β q :=
-  Quot.recₓ f h q
+  Quot.rec f h q
 
 @[reducible, elab_as_eliminator]
-protected def recOn (q : Quotientₓ s) (f : ∀ a, β (⟦a⟧))
-    (h : ∀ a b : α p : a ≈ b, (Eq.ndrec (f a) (Quotientₓ.sound p) : β (⟦b⟧)) = f b) : β q :=
-  Quot.recOnₓ q f h
+protected def recOn (q : Quotientₓ s) (f : ∀ a, β ⟦a⟧)
+    (h : ∀ a b : α p : a ≈ b, (Eq.ndrec (f a) (Quotientₓ.sound p) : β ⟦b⟧) = f b) : β q :=
+  Quot.recOn q f h
 
 @[reducible, elab_as_eliminator]
-protected def recOnSubsingleton [h : ∀ a, Subsingleton (β (⟦a⟧))] (q : Quotientₓ s) (f : ∀ a, β (⟦a⟧)) : β q :=
-  @Quot.recOnSubsingletonₓ _ _ _ h q f
+protected def recOnSubsingleton [h : ∀ a, Subsingleton (β ⟦a⟧)] (q : Quotientₓ s) (f : ∀ a, β ⟦a⟧) : β q :=
+  @Quot.recOnSubsingleton _ _ _ h q f
 
 @[reducible, elab_as_eliminator]
-protected def hrecOn (q : Quotientₓ s) (f : ∀ a, β (⟦a⟧)) (c : ∀ a b : α p : a ≈ b, HEq (f a) (f b)) : β q :=
-  Quot.hrecOnₓ q f c
+protected def hrecOn (q : Quotientₓ s) (f : ∀ a, β ⟦a⟧) (c : ∀ a b : α p : a ≈ b, HEq (f a) (f b)) : β q :=
+  Quot.hrecOn q f c
 
 end
 
@@ -188,18 +186,18 @@ protected def liftOn₂ (q₁ : Quotientₓ s₁) (q₂ : Quotientₓ s₂) (f :
   Quotientₓ.lift₂ f c q₁ q₂
 
 @[elab_as_eliminator]
-protected theorem ind₂ {φ : Quotientₓ s₁ → Quotientₓ s₂ → Prop} (h : ∀ a b, φ (⟦a⟧) (⟦b⟧)) (q₁ : Quotientₓ s₁)
+protected theorem ind₂ {φ : Quotientₓ s₁ → Quotientₓ s₂ → Prop} (h : ∀ a b, φ ⟦a⟧ ⟦b⟧) (q₁ : Quotientₓ s₁)
     (q₂ : Quotientₓ s₂) : φ q₁ q₂ :=
   Quotientₓ.ind (fun a₁ => Quotientₓ.ind (fun a₂ => h a₁ a₂) q₂) q₁
 
 @[elab_as_eliminator]
 protected theorem induction_on₂ {φ : Quotientₓ s₁ → Quotientₓ s₂ → Prop} (q₁ : Quotientₓ s₁) (q₂ : Quotientₓ s₂)
-    (h : ∀ a b, φ (⟦a⟧) (⟦b⟧)) : φ q₁ q₂ :=
+    (h : ∀ a b, φ ⟦a⟧ ⟦b⟧) : φ q₁ q₂ :=
   Quotientₓ.ind (fun a₁ => Quotientₓ.ind (fun a₂ => h a₁ a₂) q₂) q₁
 
 @[elab_as_eliminator]
 protected theorem induction_on₃ [s₃ : Setoidₓ φ] {δ : Quotientₓ s₁ → Quotientₓ s₂ → Quotientₓ s₃ → Prop}
-    (q₁ : Quotientₓ s₁) (q₂ : Quotientₓ s₂) (q₃ : Quotientₓ s₃) (h : ∀ a b c, δ (⟦a⟧) (⟦b⟧) (⟦c⟧)) : δ q₁ q₂ q₃ :=
+    (q₁ : Quotientₓ s₁) (q₂ : Quotientₓ s₂) (q₃ : Quotientₓ s₃) (h : ∀ a b c, δ ⟦a⟧ ⟦b⟧ ⟦c⟧) : δ q₁ q₂ q₃ :=
   Quotientₓ.ind (fun a₁ => Quotientₓ.ind (fun a₂ => Quotientₓ.ind (fun a₃ => h a₁ a₂ a₃) q₃) q₂) q₁
 
 end
@@ -218,6 +216,7 @@ private def rel (q₁ q₂ : Quotientₓ s) : Prop :=
       (Iff.intro (fun a₁a₂ => Setoidₓ.trans (Setoidₓ.symm a₁b₁) (Setoidₓ.trans a₁a₂ a₂b₂)) fun b₁b₂ =>
         Setoidₓ.trans a₁b₁ (Setoidₓ.trans b₁b₂ (Setoidₓ.symm a₂b₂)))
 
+-- mathport name: «expr ~ »
 local infixl:50 " ~ " => Rel
 
 private theorem rel.refl : ∀ q : Quotientₓ s, q ~ q := fun q => Quot.induction_on q fun a => Setoidₓ.refl a
@@ -239,8 +238,8 @@ variable [s₁ : Setoidₓ α] [s₂ : Setoidₓ β]
 include s₁ s₂
 
 @[reducible, elab_as_eliminator]
-protected def recOnSubsingleton₂ {φ : Quotientₓ s₁ → Quotientₓ s₂ → Sort u_c} [h : ∀ a b, Subsingleton (φ (⟦a⟧) (⟦b⟧))]
-    (q₁ : Quotientₓ s₁) (q₂ : Quotientₓ s₂) (f : ∀ a b, φ (⟦a⟧) (⟦b⟧)) : φ q₁ q₂ :=
+protected def recOnSubsingleton₂ {φ : Quotientₓ s₁ → Quotientₓ s₂ → Sort u_c} [h : ∀ a b, Subsingleton (φ ⟦a⟧ ⟦b⟧)]
+    (q₁ : Quotientₓ s₁) (q₂ : Quotientₓ s₂) (f : ∀ a b, φ ⟦a⟧ ⟦b⟧) : φ q₁ q₂ :=
   @Quotientₓ.recOnSubsingleton _ s₁ (fun q => φ q q₂) (fun a => Quotientₓ.ind (fun b => h a b) q₂) q₁ fun a =>
     Quotientₓ.recOnSubsingleton q₂ fun b => f a b
 
