Leanbin/Init/Control/Functor.lean
@@ -16,10 +16,12 @@ class Functor (f : Type u → Type v) : Type max (u + 1) v where
   map : ∀ {α β : Type u}, (α → β) → f α → f β
   mapConst : ∀ {α β : Type u}, α → f β → f α := fun α β => map ∘ const β
 
+-- mathport name: «expr <$ »
 infixr:100 " <$ " => Functor.mapConst
 
 @[reducible]
 def Functor.mapConstRev {f : Type u → Type v} [Functor f] {α β : Type u} : f β → α → f α := fun a b => b <$ a
 
+-- mathport name: «expr $> »
 infixr:100 " $> " => Functor.mapConstRev
 
