Leanbin/Init/Funext.lean
@@ -21,6 +21,7 @@ namespace Function
 protected def Equiv (f₁ f₂ : ∀ x : α, β x) : Prop :=
   ∀ x, f₁ x = f₂ x
 
+-- mathport name: «expr ~ »
 local infixl:50 " ~ " => Function.Equiv
 
 protected theorem Equiv.refl (f : ∀ x : α, β x) : f ~ f := fun x => rfl
@@ -57,10 +58,11 @@ attribute [local instance] fun_setoid
 
 /-- Function extensionality, proven using quotients. -/
 theorem funext {f₁ f₂ : ∀ x : α, β x} (h : ∀ x, f₁ x = f₂ x) : f₁ = f₂ :=
-  show extfunApp (⟦f₁⟧) = extfunApp (⟦f₂⟧) from congr_argₓ extfunApp (sound h)
+  show extfunApp ⟦f₁⟧ = extfunApp ⟦f₂⟧ from congr_argₓ extfunApp (sound h)
 
 attribute [intro!] funext
 
+-- mathport name: «expr ~ »
 local infixl:50 " ~ " => Function.Equiv
 
 instance Pi.subsingleton [∀ a, Subsingleton (β a)] : Subsingleton (∀ a, β a) :=
