Leanbin/Init/Meta/Converter/Interactive.lean
@@ -202,6 +202,7 @@ open Interactive.Types
 
 open Tactic
 
+-- mathport name: «expr ?»
 local postfix:1024 "?" => optionalₓ
 
 private unsafe def conv_at (h_name : Name) (c : conv Unit) : tactic Unit := do
