Leanbin/Init/Meta/InstanceCache.lean
@@ -21,8 +21,10 @@ open Lean.Parser
 
 open Interactive Interactive.Types
 
+-- mathport name: «expr ?»
 local postfix:1024 "?" => optionalₓ
 
+-- mathport name: «expr *»
 local postfix:1024 "*" => many
 
 namespace Tactic
