Leanbin/Init/Meta/Smt/Interactive.lean
@@ -46,8 +46,10 @@ open _Root_.Interactive
 
 open Interactive.Types
 
+-- mathport name: «expr ?»
 local postfix:1024 "?" => optionalₓ
 
+-- mathport name: «expr *»
 local postfix:1024 "*" => many
 
 unsafe def itactic : Type :=
