Leanbin/Init/Meta/Tactic.lean
@@ -95,8 +95,10 @@ open Tactic
 
 open TacticResult
 
+-- mathport name: «expr >>=[tactic] »
 infixl:2 " >>=[tactic] " => interaction_monad_bind
 
+-- mathport name: «expr >>[tactic] »
 infixl:2 " >>[tactic] " => interaction_monad_seq
 
 unsafe instance : Alternativeₓ tactic :=
@@ -1696,7 +1698,7 @@ unsafe def funext_lst (ids : List Name) : tactic Unit :=
 
 private unsafe def get_undeclared_const (env : environment) (base : Name) : ℕ → Name
   | i =>
-    let n := base <.> ("_aux_" ++ reprₓ i)
+    let n := mkStrName base ("_aux_" ++ reprₓ i)
     if ¬env.contains n then n else get_undeclared_const (i + 1)
 
 unsafe def new_aux_decl_name : tactic Name := do
